Reification/Formula.v
@@ -1,0 +1,145 @@
+(* Formulas. *)
+Inductive formula : Type :=
+    | fFalse : formula
+    | fTrue : formula
+    | fVar : Prop -> formula
+    | fNot : formula -> formula
+    | fAnd : formula -> formula -> formula
+    | fOr : formula -> formula -> formula
+    | fImpl : formula -> formula -> formula.
+
+Fixpoint formulaDenote (f : formula) : Prop :=
+match f with
+    | fFalse => False
+    | fTrue => True
+    | fVar P => P
+    | fNot f' => ~ formulaDenote f'
+    | fAnd f1 f2 => formulaDenote f1 /\ formulaDenote f2
+    | fOr f1 f2 => formulaDenote f1 \/ formulaDenote f2
+    | fImpl f1 f2 => formulaDenote f1 -> formulaDenote f2
+end.
+
+Function simpFormula (f : formula) : formula :=
+match f with
+    | fFalse => fFalse
+    | fTrue => fTrue
+    | fVar P => fVar P
+    | fNot f' =>
+        match simpFormula f' with
+            | fFalse => fTrue
+            | fTrue => fFalse
+            | f'' => fNot f''
+        end
+    | fAnd f1 f2 =>
+        match simpFormula f1, simpFormula f2 with
+            | fOr f11 f12, f2' => fOr (fAnd f11 f2') (fAnd f12 f2')
+            | f1', fOr f21 f22 => fOr (fAnd f1' f21) (fAnd f1' f22)
+            | fFalse, _ => fFalse
+            | _, fFalse => fFalse
+            | fTrue, f2' => f2'
+            | f1', fTrue => f1'
+            | f1', f2' => fAnd f1' f2'
+        end
+    | fOr f1 f2 =>
+        match simpFormula f1, simpFormula f2 with
+            | fAnd f11 f12, f2' => fAnd (fOr f11 f2') (fOr f12 f2')
+            | f1', fAnd f21 f22 => fAnd (fOr f1' f21) (fOr f1' f22)
+            | fFalse, f2' => f2'
+            | f1', fFalse => f1'
+            | fTrue, _ => fTrue
+            | _, fTrue => fTrue
+            | f1', f2' => fOr f1' f2'
+        end
+    | fImpl f1 f2 =>
+        match simpFormula f1 with
+            | fFalse => fTrue
+            | fTrue => f2
+            | fAnd f11 f12 => fImpl f11 (fImpl f12 f2)
+            | fOr f11 f12 => fAnd (fImpl f11 f2) (fImpl f12 f2)
+            | f1' => fImpl f1' f2
+        end
+end.
+
+Theorem simpFormula_correct :
+  forall f : formula, formulaDenote (simpFormula f) <-> formulaDenote f.
+Proof.
+  intros. functional induction simpFormula f; cbn.
+  Time all: try tauto.
+  repeat match goal with
+      | : nat -> _, IH : forall' : nat -> _, _ |- _ =>
+          specialize (IH)
+      | e : simpFormula ?f = _,
+        IH : formulaDenote _ (simpFormula ?f) <-> _ |- _ =>
+        rewrite <- IH, e; cbn
+  end; try (tauto; fail).
+    assert (eqExpDenote (simpHypEq (E e1 e2)) =
+           (expDenote e1' = expDenote e2')).
+      rewrite e0. cbn. trivial.
+      rewrite <- H. rewrite simpHypEq_correct. cbn. reflexivity.
+    assert (eqExpDenote (simpHypEq (E e1 e2)) <->
+            eqExpDenote (E e1' e2')).
+      rewrite e3. tauto.
+      rewrite simpHypEq_correct in H. cbn in H. tauto.
+Qed.
+
+Definition list_eq :
+  forall (l1 l2 : list nat), {l1 = l2} + {l1 <> l2}.
+Proof.
+  do 2 decide equality.
+Defined.
+
+Fixpoint solveFormula
+  {X : UCRing} (env : nat -> X) (f : formula)
+  : option (formulaDenote f).
+Proof.
+  destruct f; cbn.
+    apply None.
+    apply Some. trivial.
+    apply None.
+      destruct (exp_eq_dec (simplifyExp e) (simplifyExp e0)).
+        rewrite <- (simplifyExp_correct e),
+                <- (simplifyExp_correct e0).
+          rewrite e1. apply Some. trivial.
+        apply None.
+    apply None.
+    destruct (solveFormula X f1), (solveFormula X f2).
+      apply Some. split; assumption.
+      1-3: apply None.
+    destruct (solveFormula X f1).
+      apply Some. left. assumption.
+      destruct (solveFormula X f2).
+        apply Some. right. assumption.
+        apply None.
+    destruct (solveFormula X f2).
+      apply Some. intro. assumption.
+      apply None.
+Defined.
+
+Theorem solveFormula_correct :
+  forall (X : UCRing) (env : nat -> X) (f : formula),
+    (exists p : formulaDenote f, solveFormula f = Some p) ->
+      formulaDenote f.
+Proof.
+  intros. destruct H. assumption.
+Qed.
+
+(* Basic tactics for manipulating lists. *)
+Ltac inList x l :=
+match l with
+    | [] => false
+    | x :: _ => true
+    | _ :: ?l' => inList x l'
+end.
+
+Ltac addToList x l :=
+  let b := inList x l in
+match b with
+    | true => l
+    | false => constr:(x :: l)
+end.
+
+Ltac lookup x l :=
+match l with
+    | x :: _ => constr:(0%nat)
+    | _ :: ?l' => let n := lookup x l' in constr:(S n)
+end.
